Implement a first version of mk_update_last with assumptions

code/hash/Hacl.Hash.Blake2.fst
@@ -6,6 +6,8 @@ module ST = FStar.HyperStack.ST
 module M = LowStar.Modifies
 module S = FStar.Seq
 module U32 = FStar.UInt32
+module U64 = FStar.UInt64
+module U128 = FStar.UInt128
 
 open Lib.IntTypes
 
@@ -22,6 +24,7 @@ open FStar.Mul
 
 #push-options "--fuel 1 --ifuel 1 --z3rlimit 200"
 
+(*** update_multi *)
 noextract inline_for_extraction
 val mk_update_multi: a:hash_alg{is_blake a} -> update:update_st a -> update_multi_st a
 
@@ -70,107 +73,84 @@ let mk_update_multi a update s ev blocks n_blocks =
   C.Loops.for 0ul n_blocks inv f;
   add_extra_i a ev n_blocks
 
+(*** update_last *)
+
 noextract inline_for_extraction
-val mk_update_last: a:hash_alg{is_blake a} -> update_multi_st a -> update_last_st a
+val split (a : hash_alg{is_blake a}) (input_len : size_t) :
+  Pure (size_t & size_t & size_t)
+  (requires True)
+  (ensures fun (blocks_n, blocks_len, rest_len) ->
+    U32.v blocks_len == U32.v blocks_n * block_length a /\
+    (U32.v blocks_n, U32.v rest_len) == Spec.Blake2.split (to_blake_alg a) (U32.v input_len))
 
-let mk_update_last a update_multi s ev prev_len input input_len =
-  ST.push_frame ();
-  let h0 = ST.get () in
-
-  (* Get a series of complete blocks. *)
+let split a input_len =
   let blocks_n = U32.(input_len /^ block_len a) in
   let blocks_len = U32.(blocks_n *^ block_len a) in
-  assert (U32.v blocks_len % block_length a = 0);
-  let blocks = B.sub input 0ul blocks_len in
-
-  let ev' = update_multi s ev blocks blocks_n in
-
-  let h1 = ST.get () in
-
-  assert (S.equal (as_seq h1 s) (fst (Spec.Agile.Hash.update_multi a (as_seq h0 s, ev) (B.as_seq h0 blocks))));
-
   let rest_len = U32.(input_len -^ blocks_len) in
-
-  calc (==) {
-    v rest_len % block_length a;
-    (==) { }
-    ((v input_len - v blocks_len) % pow2 64) % block_length a;
-    (==) {
-      assert_norm (block_length Blake2S == pow2 6);
-      assert_norm (block_length Blake2B == pow2 7);
-      FStar.Math.Lemmas.pow2_modulo_modulo_lemma_1 (v input_len - v blocks_len) 6 64;
-      FStar.Math.Lemmas.pow2_modulo_modulo_lemma_1 (v input_len - v blocks_len) 6 64
-      }
-    (v input_len - v blocks_len) % block_length a;
-    (==) { FStar.Math.Lemmas.lemma_mod_sub_distr (v input_len) (v blocks_len) (block_length a) }
-    v input_len % block_length a;
-  };
-
-  calc (==) {
-    (block_length a - (len_v a prev_len + v input_len) ) % block_length a;
-    (==) { FStar.Math.Lemmas.lemma_mod_sub_distr (block_length a - v input_len) (len_v a prev_len) (block_length a) }
-    (block_length a - v input_len) % block_length a;
-    (==) { FStar.Math.Lemmas.lemma_mod_sub_distr (block_length a) (v input_len) (block_length a) }
-    (block_length a - (v input_len % block_length a)) % block_length a;
-    (==) { }
-    (block_length a - (v rest_len % block_length a)) % block_length a;
-    (==) { FStar.Math.Lemmas.lemma_mod_sub_distr (block_length a) (v rest_len) (block_length a) }
-    (block_length a - v rest_len) % block_length a;
-  };
-
-  (* The rest that doesn't make up a complete block *)
-  if rest_len = 0ul then
-    (assert (Spec.Hash.PadFinish.pad a (len_v a prev_len + v input_len) `Seq.equal` Seq.empty);
-     assert (S.equal
-      (B.as_seq h0 input `Seq.append` (Spec.Hash.PadFinish.pad a (len_v a prev_len + v input_len)))
-      (B.as_seq h1 blocks));
-    ST.pop_frame();
-    ev'
-    )
-  else (
-    let rest = B.sub input blocks_len rest_len in
+  if U32.(rest_len =^ 0ul) && U32.(blocks_n >^ 0ul) then
+    begin
+    let blocks_n = U32.(blocks_n -^ 1ul) in
+    let blocks_len = U32.(blocks_len -^ block_len a) in
+    let rest_len = block_len a in
+    blocks_n, blocks_len, rest_len
+    end
+  else blocks_n, blocks_len, rest_len
 
 
-    let pad_len = U32.(block_len a -^ rest_len) in
+(* The stateful signature for [Spec.Blake2.blake2_update_last], but where
+ * the input is actually the remaining data (smaller than a block) *)
+noextract inline_for_extraction
+let blake2_update_last_block_st (a : hash_alg{is_blake a}) =
+  s:state a ->
+  ev:extra_state a ->
+  input:B.buffer uint8 ->
+  input_len:size_t { B.length input == v input_len /\ v input_len <= block_length a /\
+                     (v #U64 #SEC ev) + v input_len <= max_input a } ->
+  ST.Stack (extra_state a)
+    (requires (fun h ->
+      B.live h s /\ B.live h input /\ B.disjoint s input))
+    (ensures (fun h0 ev' h1 ->
+      B.(modifies (loc_buffer s) h0 h1) /\
+      as_seq h1 s ==
+        Spec.Blake2.blake2_update_last (to_blake_alg a) (v #U64 #SEC ev)
+                                       (v input_len) (B.as_seq h0 input) (as_seq h0 s)))
 
-    let tmp = B.alloca (Lib.IntTypes.u8 0) (block_len a) in
-    let tmp_rest = B.sub tmp 0ul rest_len in
-    let tmp_pad = B.sub tmp rest_len pad_len in
-    B.blit rest 0ul tmp_rest 0ul rest_len;
+(* TODO: ajouter Spec.Blake2.blake2_update_last: *)
 
-    calc (==) {
-      (block_length a - (len_v a prev_len + v input_len) ) % block_length a;
-      (==) { }
-      (block_length a - v rest_len) % block_length a;
-      (==) { FStar.Math.Lemmas.small_mod (block_length a - v rest_len) (block_length a) }
-      block_length a - v rest_len;
-      (==) { assert_norm (block_length a <= pow2 32); FStar.Math.Lemmas.small_mod (block_length a - v rest_len) (pow2 32) }
-      v pad_len;
-    };
+noextract inline_for_extraction
+val mk_update_last: a:hash_alg{is_blake a} -> update_multi_st a ->
+                    blake2_update_last_block_st a -> update_last_st a
 
-    let h2 = ST.get() in
-
-    calc (==) {
-      B.as_seq h0 blocks `Seq.append` B.as_seq h2 tmp;
-      (==) { assert (Seq.equal (B.as_seq h2 tmp) (B.as_seq h2 tmp_rest `Seq.append` B.as_seq h2 tmp_pad)) }
-      B.as_seq h0 blocks `Seq.append` (B.as_seq h2 tmp_rest `Seq.append` B.as_seq h2 tmp_pad);
-      (==) { Seq.append_assoc (B.as_seq h0 blocks) (B.as_seq h2 tmp_rest) (B.as_seq h2 tmp_pad) }
-      (B.as_seq h0 blocks `Seq.append` B.as_seq h2 tmp_rest) `Seq.append` B.as_seq h2 tmp_pad;
-      (==) { assert (S.equal (B.as_seq h0 input) (S.append (B.as_seq h0 blocks) (B.as_seq h2 tmp_rest))) }
-      B.as_seq h0 input `Seq.append` B.as_seq h2 tmp_pad;
-      (==) { assert (B.as_seq h2 tmp_pad `S.equal` Spec.Hash.PadFinish.pad a (len_v a prev_len + v input_len)) }
-      B.as_seq h0 input `Seq.append` Spec.Hash.PadFinish.pad a (len_v a prev_len + v input_len);
-    };
-
-    let ev_f = update_multi s ev' tmp 1ul in
-
-    let h3 = ST.get() in
-
-    Spec.Hash.Lemmas.update_multi_associative a (as_seq h0 s, ev) (B.as_seq h0 blocks) (B.as_seq h2 tmp);
-
-    ST.pop_frame();
-    ev_f
-  )
+let mk_update_last a update_multi blake2_update_last_block s ev prev_len input input_len =
+  ST.push_frame ();
+  (**) let h0 = ST.get () in
+  (**) let input_v : Ghost.erased _ = B.as_seq h0 input in
+  (* Compute the lengths to split the blocks *)
+  let blocks_n, blocks_len, rest_len = split a input_len in
+  (* Call update_multi on the longest series of complete blocks *)
+  (**) assert (U32.v blocks_len % block_length a = 0);
+  let blocks = B.sub input 0ul blocks_len in
+  (**) let blocks_v : Ghost.erased _ = B.as_seq h0 blocks in
+  (**) assert(
+         let blocks_s, _, rem_s = Spec.Hash.Incremental.last_split_blake a input_v in
+         blocks_v `Seq.equal` blocks_s /\ v rest_len == rem_s);
+  let ev' = update_multi s ev blocks blocks_n in
+  assume(v #U64 #SEC ev' == v #U64 #SEC ev + v blocks_len);
+  assume(v #U64 #SEC ev == len_v a prev_len);
+  let h1 = ST.get () in
+  (**) assert (S.equal (as_seq h1 s)
+               (fst (Spec.Agile.Hash.update_multi a (as_seq h0 s, ev) (B.as_seq h0 blocks))));
+  (* Call update_block on the last padded block *)
+  let rest = B.sub input blocks_len rest_len in
+  (**) let rest_v : Ghost.erased _ = B.as_seq h0 rest in
+  let ev_f = blake2_update_last_block s ev' rest rest_len in
+  (**) let h2 = ST.get () in
+  (**) assert(rest_v `Seq.equal` Seq.slice input_v (v blocks_len) (v input_len));
+  (**) assert(as_seq h2 s  `Seq.equal`
+         fst (Spec.Hash.Incremental.update_last_blake a (as_seq h0 s, ev)
+         (len_v a prev_len) input_v));
+  ST.pop_frame ();
+  u64 0
 #pop-options
 
 let update_multi_blake2s: update_multi_st Blake2S =
